Clase5.Listas.fst
@@ -11,17 +11,27 @@ let rec sum_int xs =
 (* Demuestre que sum_int "distribuye" sobre la concatenación de listas. *)
 let rec sum_append (l1 l2 : list int)
   : Lemma (sum_int (l1 @ l2) == sum_int l1 + sum_int l2)
-  = admit()
+= match l1 with
+  | [] -> ()
+  | x::xs -> sum_append xs l2
 
 (* Idem para length, definida en la librería de F*. *)
 let rec len_append (l1 l2 : list int)
   : Lemma (length (l1 @ l2) == length l1 + length l2)
-  = admit()
+= match l1 with
+  | [] -> ()
+  | x::xs -> len_append xs l2
 
 let rec snoc (xs : list int) (x : int) : list int =
   match xs with
   | [] -> [x]
   | y::ys -> y :: snoc ys x
+
+let rec snoc_append (xs ys : list int) (x : int)
+  : Lemma (snoc (xs @ ys) x == xs @ snoc ys x)
+= match xs with
+  | [] -> ()
+  | z::zs' ->  snoc_append zs' ys x
 
 (* unit-tests *)
 let _ = assert (snoc [1;2;3] 4 == [1;2;3;4])
@@ -32,14 +42,33 @@ let rec rev_int (xs : list int) : list int =
   | [] -> []
   | x::xs' -> snoc (rev_int xs') x
 
-let rev_append_int (xs ys : list int)
+let rec rev_append_int (xs ys : list int)
   : Lemma (rev_int (xs @ ys) == rev_int ys @ rev_int xs)
-= admit()
+= match xs with
+  | [] -> ()
+  | x::xs' ->
+    rev_append_int xs' ys;
+    snoc_append (rev_int ys) (rev_int xs') x;
+    ()
 
-let rev_rev (xs : list int)
+let rec rev_soc (xs : list int) (x : int)
+  : Lemma (rev_int (snoc xs x) == x::rev_int xs)
+= match xs with
+  | [] -> ()
+  | z::zs -> rev_soc zs x
+
+let rec rev_rev (xs : list int)
   : Lemma (rev_int (rev_int xs) == xs)
-= admit()
+= match xs with
+  | [] -> ()
+  | x::xs' ->
+    rev_soc (rev_int xs') x;
+    rev_rev xs'
 
 let rev_injective (xs ys : list int)
   : Lemma (requires rev_int xs == rev_int ys) (ensures xs == ys)
-= admit()
+= match xs with
+  | [] -> ()
+  | x::xs' ->
+    rev_rev xs;
+    rev_rev ys
